prove logic_exchange_with_extra_guard

src/guarding/conjunct_own_rule.v
@@ -362,7 +362,288 @@ Proof using A Disc i Σ.
     setoid_rewrite <- X.
     trivial.
 Qed.
+
+Lemma uPred_ownM_andsep_to_sepand (x y: iResUR Σ) (P : iProp Σ)
+  (cond: ∀ n (p1 p2 : iResUR Σ) , (✓{n} (p1 ⋅ p2)) -> (x ≼{n} p1 ⋅ p2) -> (y ≼{n} p1) ->
+      ∃ m , y ⋅ m ≡{n}≡ p1 /\ x ≼{n} m ⋅ p2)
+  : (uPred_ownM x ∧ (uPred_ownM y ∗ P)) ⊢ (uPred_ownM y ∗ (uPred_ownM x ∧ P)).
+Proof.
+  uPred.unseal.
+  split.
+  intros n p val t.
+  unfold uPred_holds, uPred_and_def in t.
+  destruct t as [tx s].
+  unfold uPred_holds, uPred_ownM_def in tx.
+  unfold uPred_holds, uPred_sep_def in s.
+  destruct s as [p1 [p2 [eq [ty tp]]]].
+  unfold uPred_holds, uPred_ownM_def in ty.
   
+  unfold uPred_holds, uPred_sep_def.
+  
+  assert (✓{n} (p1 ⋅ p2)) as val2. { setoid_rewrite <- eq. trivial. }
+  assert (x ≼{n} (p1 ⋅ p2)) as incl2. { setoid_rewrite <- eq. trivial. }
+  
+  have k := cond n p1 p2 val2 incl2 ty.
+  destruct k as [m [ym xle]].
+  
+  exists y. exists (m ⋅ p2).
+  
+  split.
+  { setoid_rewrite eq. setoid_rewrite <- ym. rewrite cmra_assoc. trivial. }
+  split.
+  { unfold uPred_holds, uPred_ownM_def. trivial. }
+  unfold uPred_holds, uPred_and_def. split.
+  { unfold uPred_holds, uPred_ownM_def. trivial. }
+  apply (uPred_mono _ _ n n p2); trivial.
+  unfold includedN. exists m. rewrite cmra_comm. trivial.
+Qed.
+
+(*Lemma isRes_singleton_incl_from_dotquestionmark  γ (x: A) (m: option A) n j
+  (cond1 : iRes_singleton γ (x ⋅? m) ≼{n} j)
+  : iRes_singleton γ x ≼{n} j.
+Proof.
+  destruct m.
+  { replace (x ⋅? Some c) with (x ⋅ c) in cond1 by trivial.
+    generalize cond1.
+    rewrite iRes_singleton_op.
+    intro X.
+    unfold includedN in X. destruct X as [z X].
+    unfold includedN. exists (iRes_singleton γ c ⋅ z). 
+    setoid_rewrite X. symmetry. rewrite cmra_assoc. trivial.
+  }
+  replace (x ⋅? None) with x in cond1 by trivial.
+    unfold includedN in cond1. destruct cond1 as [z X].
+    unfold includedN. exists z. 
+    trivial.
+Qed.*)
+
+Lemma none_dot (a: option A) : None ⋅ a = a.
+  Proof. destruct a; trivial. Qed.
+  
+Lemma dot_none (a: option A) : a ⋅ None = a.
+  Proof. destruct a; trivial. Qed.
+  
+Lemma some_dot_some (a b: A) : (Some a) ⋅ (Some b) = (Some (a ⋅ b)).
+  Proof. trivial. Qed.
+
+Lemma le_stuff (a b c d : iResUR Σ) n
+  (t : a ⋅ b ≼{n} c)
+  : a ≼{n} d ⋅ c.
+Proof.
+  destruct t as [z t]. exists (b ⋅ z ⋅ d). setoid_rewrite t.
+  setoid_replace (d ⋅ (a ⋅ b ⋅ z)) with ((a ⋅ b ⋅ z) ⋅ d) by (apply cmra_comm).
+  setoid_replace (a ⋅ ((b ⋅ z) ⋅ d)) with ((a ⋅ (b ⋅ z)) ⋅ d) by (apply cmra_assoc).
+  setoid_replace (a ⋅ (b ⋅ z)) with (a ⋅ b ⋅ z) by (apply cmra_assoc).
+  trivial.
+Qed.
+  
+Lemma le_stuff2 (a c d : iResUR Σ) n
+  (t : a ≼{n} c)
+  : a ≼{n} d ⋅ c.
+Proof.
+  destruct t as [z t]. exists (z ⋅ d). setoid_rewrite t.
+  setoid_replace (d ⋅ (a ⋅ z)) with ((a ⋅ z) ⋅ d) by (apply cmra_comm).
+  setoid_rewrite <- cmra_assoc. trivial.
+Qed.
+
+Lemma incl_l (b b' c: iResUR Σ) n
+  (t: b ≼{n} b') : b ⋅ c ≼{n} b' ⋅ c.
+Proof.
+  destruct t as [z t]. exists z. setoid_rewrite t.
+  setoid_replace (b ⋅ z ⋅ c) with (b ⋅ (z ⋅ c)) by (symmetry; apply cmra_assoc).
+  setoid_replace (b ⋅ c ⋅ z) with (b ⋅ (c ⋅ z)) by (symmetry; apply cmra_assoc).
+  setoid_replace (c ⋅ z) with (z ⋅ c) by (apply cmra_comm). trivial.
+Qed.
+
+Lemma incl_r (b b' c: iResUR Σ) n
+  (t: b ≼{n} b') : c ⋅ b ≼{n} c ⋅ b'.
+Proof.
+  destruct t as [z t]. exists z. setoid_rewrite t. rewrite cmra_assoc. trivial.
+Qed.
+  
+Lemma incl_stuff3 (a b c b' c' : iResUR Σ) n
+      (i1: a ≼{n} b ⋅ c) (i2: b ≼{n} b') (i3: c ≼{n} c')
+      : (a ≼{n} b' ⋅ c').
+Proof.
+  eapply cmra_includedN_trans. { apply i1. }
+  apply (cmra_includedN_trans _ (b ⋅ c) (b ⋅ c') (b' ⋅ c')).
+  - apply incl_r; trivial. - apply incl_l; trivial.
+Qed.
+      
+Lemma incl_stuff4 (a b b' c' : iResUR Σ) n
+      (i1: a ≼{n} b) (i2: b ≼{n} b')
+      : (a ≼{n} b' ⋅ c').
+Proof.
+  eapply cmra_includedN_trans. { apply i1. }
+  apply (cmra_includedN_trans _ b b' (b' ⋅ c')); trivial.
+  exists c'. trivial.
+Qed.
+  
+Lemma discrete_fun_insert_incl_iRes_singleton n (m: A) (p1: iResUR Σ) (γ: gname) :
+      (iRes_singleton γ m) ≼{n}
+  discrete_fun_insert (inG_id i)
+            (<[γ:=inG_unfold (cmra_transport inG_prf m)]> (p1 (inG_id i))) p1.
+Proof.
+    exists (discrete_fun_insert 
+        (inG_id i)
+        (delete γ (p1 (inG_id i)))
+        p1).
+    apply equiv_dist.
+    intros x'.
+    have h : Decision (inG_id i = x') by solve_decision. destruct h.
+    + setoid_rewrite discrete_fun_lookup_op. subst x'.
+      setoid_rewrite discrete_fun_lookup_singleton.
+      setoid_rewrite discrete_fun_lookup_insert.
+      intro γ0.
+      have h1 : Decision (γ = γ0) by solve_decision. destruct h1.
+      * subst γ0. rewrite lookup_op. rewrite lookup_delete.
+          rewrite lookup_insert.
+        rewrite op_None_right_id.
+        rewrite lookup_singleton. trivial.
+      * rewrite lookup_insert_ne; trivial. 
+        rewrite lookup_op.
+        rewrite lookup_singleton_ne; trivial. rewrite op_None_left_id.
+        rewrite lookup_delete_ne; trivial.
+    + setoid_rewrite discrete_fun_lookup_op.
+      setoid_rewrite discrete_fun_lookup_singleton_ne; trivial.
+      setoid_rewrite discrete_fun_lookup_insert_ne; trivial.
+      symmetry.
+      apply ucmra_unit_left_id.
+Qed.
+            
+Lemma Some_incl_Some_Some_to_iRes_singleton_incl (a b c : A) n γ
+            (sincl: Some a ≼{n} Some b ⋅ Some c) :
+            (iRes_singleton γ a ≼{n} iRes_singleton γ b ⋅ iRes_singleton γ c).
+Proof.
+  rewrite <- iRes_singleton_op. destruct sincl as [z sincl]. destruct z.
+  + rewrite some_dot_some in sincl. rewrite some_dot_some in sincl. inversion sincl.
+    exists (iRes_singleton γ c0). rewrite <- iRes_singleton_op.
+    unfold iRes_singleton. f_equiv. apply: singletonM_proper. setoid_rewrite H1. trivial.
+  + rewrite some_dot_some in sincl. rewrite dot_none in sincl. inversion sincl.
+    exists ε. rewrite ucmra_unit_right_id.
+    unfold iRes_singleton. f_equiv. apply: singletonM_proper. setoid_rewrite H1. trivial.
+Qed.
+            
+Lemma Some_incl_Some_None_to_iRes_singleton_incl (a b : A) n γ
+            (sincl: Some a ≼{n} Some b ⋅ None) :
+            (iRes_singleton γ a ≼{n} iRes_singleton γ b).
+Proof.
+  destruct sincl as [z sincl]. rewrite dot_none in sincl. destruct z.
+  + rewrite some_dot_some in sincl. inversion sincl. exists (iRes_singleton γ c).
+    rewrite <- iRes_singleton_op. unfold iRes_singleton. f_equiv. apply: singletonM_proper.
+    setoid_rewrite H1. trivial.
+  + rewrite dot_none in sincl. inversion sincl. exists ε. rewrite ucmra_unit_right_id.
+    unfold iRes_singleton. f_equiv. apply: singletonM_proper. setoid_rewrite H1. trivial.
+Qed.
+
+Lemma andsep_to_sepand γ (x y: A) (P : iProp Σ)
+  (cond: ∀ n (p1 : A) (p2 r1 r2 : option A) , (✓ (p1 ⋅? p2))
+      -> (x ⋅? r1 ≡ p1 ⋅? p2)
+      -> (y ⋅? r2 ≡ p1)
+      -> ∃ (m: option A) , y ⋅? m ≡ p1 /\ Some x ≼{n} m ⋅ p2)
+  : (own γ x ∧ (own γ y ∗ P)) ⊢ (own γ y ∗ (own γ x ∧ P)).
+Proof using A Disc i Σ.
+  rewrite own_eq. unfold own_def. apply uPred_ownM_andsep_to_sepand.
+  intros n p1 p2 val incl1 incl2.
+  
+  unfold includedN in incl1. destruct incl1 as [z1 incl1].
+  unfold includedN in incl2. destruct incl2 as [z2 incl2].
+  
+  assert (project (p1 ⋅ p2) γ ≡{n}≡ project (iRes_singleton γ x ⋅ z1) γ) as X.
+    { apply proper_project_equiv_n; trivial. }
+    
+  assert (project p1 γ ≡{n}≡ project (iRes_singleton γ y ⋅ z2) γ) as Y.
+    { apply proper_project_equiv_n; trivial. }
+  
+  setoid_rewrite project_op in X.
+  setoid_rewrite project_iRes_singleton in X.
+  
+  setoid_rewrite project_op in Y.
+  setoid_rewrite project_iRes_singleton in Y.
+  
+  replace (Some x ⋅ project z1 γ) with (Some (x ⋅? project z1 γ)) in X.
+  2: { unfold "⋅?". destruct (project z1 γ); trivial. }
+  
+  replace (Some y ⋅ project z2 γ) with (Some (y ⋅? project z2 γ)) in Y.
+  2: { unfold "⋅?". destruct (project z2 γ); trivial. }
+  
+  destruct (project p1 γ) eqn:p1eqn. 2: { inversion Y. }
+  
+  inversion Y.
+  
+  replace (Some c ⋅ project p2 γ) with (Some (c ⋅? project p2 γ)) in X.
+  2: { unfold "⋅?". destruct (project p2 γ); trivial. }
+  inversion X.
+  
+  assert (✓ (c ⋅? project p2 γ)) as val2. {
+    have vp := valid_project _ γ _ val.
+    setoid_rewrite project_op in vp.
+    setoid_rewrite p1eqn in vp.
+    replace (Some c ⋅ project p2 γ) with (Some (c ⋅? project p2 γ)) in vp.
+    - unfold includedN in vp. rewrite <- cmra_discrete_valid_iff in vp. trivial.
+    - destruct (project p2 γ); trivial.
+  }
+  
+  symmetry in H4. have eq1 := discrete_equiv _ _ _ H4.
+  symmetry in H1. have eq2 := discrete_equiv _ _ _ H1.
+  have cond0 := cond n c (project p2 γ) (project z1 γ) (project z2 γ) val2 eq1 eq2.
+  destruct cond0 as [m [req_eq res_incl]].
+  destruct m as [m|].
+  2: {
+    exists z2. split.
+      + symmetry. apply incl2.
+      + unfold includedN in res_incl. destruct res_incl as [z res_incl]. destruct z.
+        * rewrite none_dot in res_incl. rewrite some_dot_some in res_incl.
+          have ri' := discrete_equiv_opt _ _ _ res_incl.
+          have t := iRes_incl_from_proj γ (x ⋅ c0) p2 n ri'.
+          setoid_rewrite iRes_singleton_op in t.
+          eapply le_stuff. apply t.
+        * rewrite none_dot in res_incl. rewrite dot_none in res_incl.
+          have ri' := discrete_equiv_opt _ _ _ res_incl.
+          have t := iRes_incl_from_proj γ x p2 n ri'.
+          eapply le_stuff2. apply t.
+  }
+  exists ((discrete_fun_insert (inG_id i) (<[ γ := inG_unfold (cmra_transport inG_prf m) ]>
+      (p1 (inG_id i))) p1)).
+  split.
+  - apply equiv_dist.
+    intros x'.
+    have h : Decision (inG_id i = x') by solve_decision. destruct h.
+    + setoid_rewrite discrete_fun_lookup_op. subst x'.
+      setoid_rewrite discrete_fun_lookup_singleton.
+      setoid_rewrite discrete_fun_lookup_insert.
+      intro γ0.
+      have h1 : Decision (γ = γ0) by solve_decision. destruct h1.
+      * subst γ0. rewrite lookup_op. rewrite lookup_insert. rewrite lookup_insert.
+        unfold "⋅", cmra_op, optionR, option_op_instance, union_with, option_union_with.
+        unfold project in p1eqn.
+        destruct (p1 (inG_id i) !! γ) eqn:p1eqn'; try discriminate.
+        inversion p1eqn.
+        rewrite p1eqn'. f_equiv.
+        rewrite <- (cmra_morphism_op _).
+        rewrite <- cmra_transport_op.
+        simpl in req_eq. setoid_rewrite req_eq. setoid_rewrite <- H6.
+        rewrite cmra_transport_trans eq_trans_sym_inv_l /=.
+        setoid_rewrite inG_unfold_fold. 
+        trivial.
+      * rewrite lookup_op. rewrite lookup_insert_ne; trivial.
+        rewrite lookup_insert_ne; trivial.
+        rewrite lookup_empty.
+        rewrite op_None_left_id.
+        trivial.
+    + setoid_rewrite discrete_fun_lookup_op.
+      setoid_rewrite discrete_fun_lookup_singleton_ne; trivial.
+      setoid_rewrite discrete_fun_lookup_insert_ne; trivial.
+      apply ucmra_unit_left_id.
+  - have ineq1 := discrete_fun_insert_incl_iRes_singleton n m p1 γ.
+    destruct (project p2 γ) eqn:p2eqn.
+    + assert (project p2 γ ≡ Some c0) as p2eqn'. { rewrite p2eqn. trivial. }
+      have ineq2 := iRes_incl_from_proj γ c0 p2 n p2eqn'.
+      have ineq3 := Some_incl_Some_Some_to_iRes_singleton_incl _ _ _ _ γ res_incl.
+      apply (incl_stuff3 _ _ _ _ _ _ ineq3 ineq1 ineq2).
+    + have ineq3 := Some_incl_Some_None_to_iRes_singleton_incl _ _ _ γ res_incl.
+      apply (incl_stuff4 _ _ _ _ _ ineq3 ineq1).
+Qed.
   
 End ConjunctOwnRule.
 
@@ -400,6 +681,44 @@ Proof using A Disc i Σ.
     unfold "⋅?" at 2. trivial.
   }
   iFrame.
+Qed.
+
+Definition opt_to_unital (x: option A) := match x with Some x' => x' | None => ε end.
+Lemma q_dot_equiv (x: A) (w: option A) : (x ⋅? w) ≡ (x ⋅ opt_to_unital w).
+Proof.
+  destruct w; trivial. unfold opt_to_unital. rewrite ucmra_unit_right_id. trivial.
+Qed.
+
+Lemma andsep_to_sepand_ucmra γ (x y: A) (P : iProp Σ)
+  (cond: ∀ (p1 p2 r1 r2 : A) , (✓ (p1 ⋅ p2))
+      -> (x ⋅ r1 ≡ p1 ⋅ p2)
+      -> (y ⋅ r2 ≡ p1)
+      -> ∃ (m: A) , y ⋅ m ≡ p1 /\ x ≼ m ⋅ p2)
+  : (own γ x ∧ (own γ y ∗ P)) ⊢ (own γ y ∗ (own γ x ∧ P)).
+Proof using A Disc i Σ.
+  apply andsep_to_sepand.
+  intros n p1 p2 r1 r2 val eq1 eq2.
+  setoid_rewrite q_dot_equiv in val.
+  setoid_rewrite q_dot_equiv in eq1.
+  setoid_rewrite q_dot_equiv in eq2.
+  have cond0 := cond p1 (opt_to_unital p2) (opt_to_unital r1) (opt_to_unital r2) val eq1 eq2.
+  destruct cond0 as [m [cond1 cond2]]. exists (Some m).
+  unfold "⋅?".
+  split; trivial.
+  destruct p2.
+  - unfold opt_to_unital in cond2.
+    unfold included in cond2. destruct cond2 as [z cond2].
+    unfold includedN. exists (Some z). 
+    unfold "⋅", cmra_op, optionR, option_op_instance, union_with, option_union_with.
+    setoid_rewrite cond2. trivial.
+  - unfold opt_to_unital in cond2.
+    unfold included in cond2. destruct cond2 as [z cond2].
+    unfold includedN. exists (Some z). 
+    unfold "⋅", cmra_op, optionR, option_op_instance, union_with, option_union_with.
+    generalize cond2.
+    rewrite ucmra_unit_right_id.
+    intro cond2'.
+    setoid_rewrite cond2'. trivial.
 Qed.
 
 End ConjunctOwnRuleU.
